Examples before cleaning

Examples.v
@@ -147,7 +147,7 @@ Proof.
   dep_destruct x1. clear x1.
   dep_destruct s0. dep_destruct s1. clear s0. clear s1.
   dep_destruct x2. clear x2.
-  dep_destruct s0. dep_destruct s1. clear s0. clear s1.
+  dep_destruct s1. dep_destruct s4. clear s1. clear s4.
   dep_destruct x1. clear x1. clear x. clear x0. cbn in x2.
     unfold decryptM in x2.
     destruct  (decrypt
@@ -156,6 +156,176 @@ Proof.
       destruct p. assumption.
       inversion x2.
   
-    inversion s1.
+    inversion s5.
 Qed.
+
+
+Definition incPayload (m:message Basic) : (message Basic) :=
+  match m with
+  | basic n => basic (n + 1)
+  | _ => bad Basic                 
+  end.
+
+Definition proto4 (payload4:(message Basic)) :=
+  send payload4;
+  x <- receive;
+  ReturnC (t:=Basic) x.
+Check proto4.
+
+Definition proto5 :=
+  x <- receive;
+  send (incPayload x);
+  ReturnC x.
+Check proto5.
+
+Example dual45 : forall x, Dual (proto4 x) proto5.
+Proof.
+  cbv.
+  split.
+  reflexivity.
+  split.
+    reflexivity.
+    trivial.
+Qed.
+
+Definition property45 : forall x4 x5 st st',
+    multi st _ _ _ (proto4 x4) proto5 (ReturnC x5) st' ->
+    x5 = incPayload x4.
+Proof.
+  intros.
+  dep_destruct H. clear H.
+  dep_destruct s0. dep_destruct s1. clear s0. clear s1.
+  dep_destruct x1. clear x1.
+  dep_destruct s0. dep_destruct s1. clear s0. clear s1.
+  dep_destruct x2. reflexivity. 
+  inversion s1.
+Qed.
+    
+    
+
+
+Definition hoare_triple{p1t p2t p3t:protoType}{t:type}
+           (P:Assertion)
+           (p1:protoExp p1t) (p2:protoExp p2t) (p3:protoExp p3t)
+           (Q:Assertion) : Prop :=
+  forall st st',
+     P st ->
+     multi st _ _ _ p1 p2 p3 st' ->
+     Q (newState st').
+
+(*Definition inPb : forall mt (m:message mt) (pf: mt = Basic) (s:State),
+    Prop.
+Proof.
+  intros. subst. destruct (my_in m s.(basics)). exact True. exact False.
+Qed.
+
+Definition inPk : forall mt (m:message mt) (pf: mt = Key) (s:State),
+    Prop.
+Proof.
+  intros. subst. destruct (my_in m s.(keys)). exact True. exact False.
+Qed.
+*)
+
+Definition inPb (m:message Basic) (s:State) :=
+  if (my_inB m s.(basics)) then True
+  else False.
+
+Definition inPk (m:message Key) (s:State) :=
+  if (my_inK m s.(keys)) then True
+  else False.
+         
+
+(*Definition inP t (m:message t) (s:State) :=
+  match t as t' return (t = t') -> Prop with
+  | Basic => fun pf => (inPb t m pf s)
+  | Key => fun pf => (inPk t m pf s)
+  | _ => fun _ => False                 
+  end (eq_refl t). 
+
+Definition notInP t (m:message t) (s:State) :=
+  ~ (inP t m s).
+ *)
+
+Definition notInPb (m:message Basic) (s:State) :=
+  ~ (inPb m s).
+
+
+
+Definition learnedB {p1t p2t p3t:protoType}
+           (m:message Basic)
+           (p1:protoExp p1t) (p2:protoExp p2t) (p3:protoExp p3t) : Prop :=
+  hoare_triple (t:=Basic) (notInPb m) p1 p2 p3 (inPb m).
+ 
+
+Definition p1 :=
+  send (basic 33);
+  EpsC.
+
+Definition p2 :=
+  x <- receive;
+  ReturnC (t:=Basic) x.
+
+Definition learnedProof : learnedB (basic 33) p2 p1 (ReturnC (basic 33)).
+Proof.
+  intros.
+  unfold p1. unfold p2. unfold learnedB. unfold hoare_triple.
+  intros.
+  dep_destruct H0. clear H0.
+  dep_destruct s0. dep_destruct s1. clear s0. clear s1.
+  dep_destruct x1. clear x1. simpl. cbn. trivial.
+  inversion s1.
+Qed.
+
+Definition p3Payload := (basic 42).
+Definition p3 :=
+  send encrypt _ p3Payload (public 0);
+  EpsC.
+
+Definition p4 :=
+  x <- receive;
+  ReturnC (t:=Encrypt Basic) x.
+
+Axiom inInfo : forall (m:message Key) (st:State),
+    inPk m st ->
+    exists kl b kob bob, st = (mkState (m :: kl) b kob bob).
+
+Definition hoare_triple'{p1t p2t p3t:protoType}{t:type} (st:State)
+           (p1:protoExp p1t) (p2:protoExp p2t) (p3:protoExp p3t)
+           (Q:Assertion) : Prop :=
+  forall st',
+     multi st _ _ _ p1 p2 p3 st' ->
+     Q (newState st').
+
+Definition notLearnedIf : hoare_triple' (t:= Encrypt Basic)
+                          emptyState
+                          p4 p3 (ReturnC (encrypt _ p3Payload (public 0)))
+                          (notInPb p3Payload).
+Proof.
+  unfold p3. unfold p4. unfold hoare_triple'.
+  intros.
+  dep_destruct H. clear H. 
+  dep_destruct s0. clear s0. dep_destruct s1. clear s1.
+  cbn in x1. 
+  dep_destruct x1. cbv. intros H. inversion H.
+  inversion s2.
+Qed.
+
+Definition learnedIf : hoare_triple' (t:= Encrypt Basic)
+                       (updateState (key (public 0)) emptyState)
+                       p4 p3 (ReturnC (encrypt _ p3Payload (public 0)))
+                       (inPb p3Payload).
+Proof.
+  unfold p3. unfold p4. unfold hoare_triple'.
+  intros.
+  dep_destruct H. clear H. 
+  dep_destruct s0. clear s0. dep_destruct s1. clear s1.
+  cbn in x1.
+  dep_destruct x1. clear x1. cbv. trivial.
+  inversion s2.
+Qed.
+
+  
+  
+  
+
 
